show extensionality of extmap

src/fmap/extensional.v
@@ -73,6 +73,84 @@ Section Sorted.
         inversion_clear H.
         congruence.
   Defined.
+
+  Local Hint Constructors NoDup.
+
+  Context (R_trans : forall a b c, R a b -> R b c -> R a c)
+          (R_antisym : forall a, R a a -> False).
+  Lemma sorted_list_nodup (l : list T) :
+    Sorted R l -> NoDup l.
+  Proof.
+    intros H.
+    eapply Sorted_StronglySorted in H; eauto using R_trans.
+    induction H as [|???? Hf]; eauto.
+    econstructor; eauto.
+    intro; eapply Forall_forall in Hf; eauto using R_antisym.
+  Qed.
+
+  Context (T_eq_lem : forall a b : T, a = b \/ a <> b).
+
+  Lemma nodup_in_cons_extend {t} a (l1 l2 : list t) :
+    NoDup (a :: l1) ->
+    (forall x, In x (a :: l1) -> In x (a :: l2)) ->
+    forall x, In x l1 -> In x l2.
+  Proof.
+    intros Hn H x ?.
+    inversion_clear Hn.
+    cbn [In] in H.
+    destruct (H x); eauto.
+    congruence.
+  Qed.
+
+  Lemma sorted_list_set (l1 l2 : list T) :
+    Sorted R l1 -> Sorted R l2 ->
+    (forall x, In x l1 <-> In x l2) ->
+    l1 = l2.
+  Proof.
+    intros HS1 HS2 HIn.
+    revert dependent l2.
+    induction l1 as [|a1]; intros.
+    - destruct l2; eauto.
+      cbn [In] in HIn.
+      exfalso.
+      eapply HIn; eauto.
+    - induction l2 as [|a2].
+      { cbn [In] in HIn.
+        exfalso.
+        eapply HIn; eauto. }
+      destruct (T_eq_lem a1 a2) as [<-|].
+      + f_equal.
+        apply IHl1; try solve [eapply Sorted_inv; eauto].
+        intros.
+        split; eapply nodup_in_cons_extend;
+          repeat (eapply HIn || eauto using sorted_list_nodup).
+      + exfalso.
+        assert (In a1 l2).
+        {
+          cbn [In] in HIn.
+          edestruct HIn.
+          intuition congruence.
+        }
+        assert (In a2 l1).
+        {
+          cbn [In] in HIn.
+          edestruct (HIn a2).
+          intuition congruence.
+        }
+        assert (R a1 a2).
+        {
+          eapply Sorted_StronglySorted in HS1; eauto using R_trans.
+          inversion_clear HS1.
+          eapply Forall_forall; eauto.
+        }
+        assert (R a2 a1).
+        {
+          eapply Sorted_StronglySorted in HS2; eauto using R_trans.
+          inversion_clear HS2.
+          eapply Forall_forall; eauto.
+        }
+        eauto using R_trans, R_antisym.
+  Qed.
 End Sorted.
 
 Section Extmap.
@@ -110,7 +188,8 @@ Section Extmap.
 
   Definition empty : extmap := exist _ nil (Sorted_nil _).
 
-  Fixpoint add' (k : key) (v : value) (l : list (key * value)) : list (key * value) :=
+  Fixpoint add' (k : key) (v : value) (l : list (key * value))
+    : list (key * value) :=
     match l with
     | nil => (k, v) :: nil
     | cons (k', v') l =>
@@ -139,7 +218,7 @@ Section Extmap.
           eauto; inversion H; eauto.
   Qed.
 
-  Lemma add_sort (k : key) (v : value) (l : list (key * value)) :
+  Lemma add_sorted (k : key) (v : value) (l : list (key * value)) :
     Sorted lt (map fst l) -> Sorted lt (map fst (add' k v l)).
     intros H.
     induction l as [|[k' v']]; cbn [add'].
@@ -149,13 +228,168 @@ Section Extmap.
           eauto; inversion H; eauto using add_hdrel.
   Qed.
 
-  (* Definition extensional : @fmap.operations key value := *)
-  (*   {| *)
-  (*     fmap.M := extmap; *)
-  (*     fmap.empty := empty; *)
-  (*     fmap.add := add; *)
-  (*     fmap.find := find; *)
-  (*     fmap.fold_ac := fold_ac; *)
-  (*   |}. *)
+  Definition add (k : key) (v : value) (m : extmap) : extmap.
+    destruct m as [l s].
+    exists (add' k v l).
+    eauto using add_sorted.
+  Defined.
 
+  Fixpoint find' k l : option value :=
+    match l with
+    | nil => None
+    | (k', v') :: l => match key_dec k k' with
+                       | left _ => Some v'
+                       | right _ => find' k l
+                       end
+    end.
+
+  Definition find (k : key) (m : extmap) : option value :=
+    let (l, _) := m in
+    find' k l.
+
+  Definition fold_ac (S : Type)
+             (f : key -> value -> S -> S) (init : S) (m : extmap) : S :=
+    let (l, _) := m in
+    List.fold_right (fun '(k, v) => f k v) init l.
+
+  Definition extensional : @fmap.operations key value :=
+    {|
+      fmap.M := extmap;
+      fmap.empty := empty;
+      fmap.add := add;
+      fmap.find := find;
+      fmap.fold_ac := fold_ac;
+    |}.
+
+  Context {lt_trans : forall a b c : key, a < b -> b < c -> a < c}
+          {lt_antisym : forall a : key, a < a -> False}.
+
+  Lemma find_in k (m : extmap) v :
+    let (l, _) := m in
+    In (k, v) l <-> match find' k l with
+                    | Some v' => v = v'
+                    | None => False
+                    end.
+  Proof.
+    destruct m as [l s].
+    induction l as [|[k' v']]; cbn [find'].
+    - split; eauto.
+    - cbn [map fst] in s.
+      destruct (key_dec k k') as [<-|].
+      + split.
+        * intros [|]; try congruence.
+          exfalso.
+          eapply sorted_list_nodup in s; eauto.
+          inversion_clear s.
+          match goal with
+          | H : ~ In k (map fst l) |- _ => change k with (fst (k, v)) in H
+          end.
+          eauto using in_map.
+        * intros <-.
+          eauto using in_eq.
+      + rewrite <- IHl; try solve [inversion s; eauto].
+        split; eauto using in_cons.
+        intros [|]; congruence.
+  Qed.
+
+  Lemma find_keys_ext (m1 m2 : extmap) :
+    let (l1, _) := m1 in
+    let (l2, _) := m2 in
+    (forall k, find' k l1 = find' k l2) ->
+    map fst l1 = map fst l2.
+  Proof.
+    destruct m1 as [l1 s1].
+    destruct m2 as [l2 s2].
+    intros Hfind.
+    eapply sorted_list_set; eauto;
+      try solve [intros; edestruct key_dec; eauto].
+    intros k.
+    specialize (Hfind k).
+    assert (forall v, In (k, v) l1 <-> In (k, v) l2) as Hf.
+    {
+      pose proof (find_in k (exist _ l1 s1)) as Hf1;
+        cbv iota beta in Hf1;
+        pose proof (find_in k (exist _ l2 s2)) as Hf2;
+        cbv iota beta in Hf2.
+      destruct (find' k l1) as [v1|];
+        destruct (find' k l2) as [v2|];
+        cbn [find']; try congruence;
+          [inversion Hfind; subst v2|];
+          setoid_rewrite Hf1;
+          setoid_rewrite Hf2;
+          intuition.
+    }
+
+    repeat rewrite in_map_iff.
+    split;
+      intros ((k'&?)&?&?);
+      cbn [fst] in *;
+      subst k';
+      exists (k, v);
+      (rewrite Hf || rewrite <- Hf); eauto.
+  Qed.
+
+  Lemma ext_cons k v l1 l2 :
+    Sorted lt (map fst ((k, v) :: l1)) ->
+    Sorted lt (map fst ((k, v) :: l2)) ->
+    (forall k', find' k' ((k, v) :: l1) = find' k' ((k, v) :: l2)) ->
+    forall k', find' k' l1 = find' k' l2.
+  Proof.
+    intros s1 s2 Hfind k'.
+    cbn [find'] in Hfind.
+    specialize (Hfind k').
+    destruct (key_dec k' k) as [->|]; eauto.
+    assert (Sorted lt (map fst l1)) as s1' by (inversion_clear s1; eauto).
+    assert (Sorted lt (map fst l2)) as s2' by (inversion_clear s2; eauto).
+    eapply sorted_list_nodup in s1; eauto.
+    eapply sorted_list_nodup in s2; eauto.
+    transitivity (None : option value);
+      [pose proof (find_in k (exist _ l1 s1')) as Hf|
+       pose proof (find_in k (exist _ l2 s2')) as Hf];
+      cbv iota beta in Hf;
+      destruct (find' k _) as [v'|]; eauto;
+        exfalso;
+        specialize (Hf v');
+        destruct Hf as [_ Hf];
+        specialize (Hf eq_refl);
+        eapply in_map with (f:=fst) in Hf;
+        cbn [map fst] in s1, s2, Hf;
+        solve [(inversion s1 + inversion s2);
+               congruence].
+  Qed.
+
+  Lemma extmap_extensional (m1 m2 : extmap) :
+    (forall k, find k m1 = find k m2) ->
+    m1 = m2.
+  Proof.
+    intros Hfind.
+    destruct m1 as [l1 s1], m2 as [l2 s2].
+    enough (l1 = l2) as <-.
+    {
+      f_equal.
+      eapply Sorted_uniq; eauto.
+    }
+    assert (map fst l1 = map fst l2) as Hmap by
+          (eapply (find_keys_ext (exist _ l1 s1) (exist _ l2 s2));
+           eauto).
+
+    cbn [find] in Hfind.
+    revert dependent l2.
+    induction l1 as [|[k1 v1]]; destruct l2 as [|[k2 v2]];
+      intros;
+      try solve [cbn [map] in Hmap; congruence].
+    assert (k1 = k2) as <- by (cbn [map fst] in Hmap; congruence).
+    assert (v1 = v2) as <-.
+    {
+      specialize (Hfind k1);
+        cbn [find'] in Hfind.
+      destruct (key_dec k1 k1); congruence.
+    }
+    f_equal.
+    assert (Sorted lt (map fst l1)) as s1' by (inversion_clear s1; eauto).
+    assert (Sorted lt (map fst l2)) as s2' by (inversion_clear s2; eauto).
+    apply IHl1; eauto using ext_cons.
+    eapply (find_keys_ext (exist _ l1 s1') (exist _ l2 s2')).
+    eauto using ext_cons.
+  Qed.
 End Extmap.
